VisualProof.lean
@@ -1,3 +1,2 @@
 import VisualProof.Rule.Soundness
 import VisualProof.Rule.Executable
-import VisualProof.Rule.Vacuity.AssemblyCompleteness
