VisualProof/Theory/Relation.lean
@@ -1,9 +1,0 @@
-namespace VisualProof.Theory
-
-abbrev RelCtx := List Nat
-
-structure RelVar (ctx : RelCtx) (arity : Nat) where
-  index : Fin ctx.length
-  hasArity : ctx.get index = arity
-
-end VisualProof.Theory
